theories/Compositional_Structures/Basic_Modules/Component_Types/Electoral_Module_Ref.thy
@@ -1,31 +1,32 @@
 theory Electoral_Module_Ref                      
-  imports "Social_Choice_Types/Profile_Array"
+  imports "Verified_Voting_Rule_Construction.Profile_List"
           "Social_Choice_Types/Result_Ref"
           "Verified_Voting_Rule_Construction.Electoral_Module"
+           Refine_Imperative_HOL.IICF
 begin                            
 
-type_synonym 'a Electoral_Module_Ref = "'a set \<Rightarrow> 'a Profile_Array \<Rightarrow> 'a Result"
+type_synonym 'a Electoral_Module_Ref = "'a set \<Rightarrow> 'a Profile_List \<Rightarrow> 'a Result"
 
 definition electoral_module_r :: " 'a Electoral_Module_Ref \<Rightarrow> bool" where
-  "electoral_module_r mr \<equiv> \<forall> A pa. finite_profile_a A pa \<longrightarrow> well_formed A (mr A pa)"
+  "electoral_module_r mr \<equiv> \<forall> A pa. well_formed A (mr A pa)"
 
 lemma em_corres:
-  fixes A :: "'a set" and pa :: "'a Profile_Array"
-  assumes "(em_r, em) \<in> (Id \<rightarrow> (br pa_to_pr (profile_a A)) \<rightarrow> Id)" 
-      and " (profile_a A pa)"
-  shows "(em_r A pa) = (em A (pa_to_pr pa))"
+  fixes A :: "'a set" and pa :: "'a Profile_List"
+  assumes "(em_r, em) \<in> (Id \<rightarrow> (br pl_to_pr_\<alpha> (profile_l A)) \<rightarrow> Id)" 
+      and " (profile_l A pa)"
+  shows "(em_r A pa) = (em A (pl_to_pr_\<alpha> pa))"
 using assms proof (-)
-  assume p: "profile_a A pa"
-  assume "(em_r, em) \<in> Id \<rightarrow> br pa_to_pr (profile_a A) \<rightarrow> Id"
-  from p this show "em_r A pa = em A (pa_to_pr pa)"
+  assume p: "profile_l A pa"
+  assume "(em_r, em) \<in> Id \<rightarrow> br pl_to_pr_\<alpha> (profile_l A) \<rightarrow> Id"
+  from p this show "em_r A pa = em A (pl_to_pr_\<alpha> pa)"
     by (metis (no_types, opaque_lifting) in_br_conv pair_in_Id_conv tagged_fun_relD_none)
 qed
 
 lemma em_onA:
   fixes A :: "'a set" 
-  assumes "(em_r A, em A) \<in> (br pa_to_pr (profile_a A)) \<rightarrow> Id" 
-    and " (profile_a A pa)"
-  shows "(em_r A pa) = (em A (pa_to_pr pa))"
+  assumes "(em_r A, em A) \<in> (br pl_to_pr_\<alpha> (profile_l A)) \<rightarrow> Id" 
+    and " (profile_l A pa)"
+  shows "(em_r A pa) = (em A (pl_to_pr_\<alpha> pa))"
   by (metis assms(1) assms(2) brI pair_in_Id_conv tagged_fun_relD_rhs)
 
 end
